and one escape lemma, one!

theories/Escape.v
@@ -1,3 +1,4 @@
+From MetaCoq Require Import PCUICAst.
 Require Import Untyped MLTTTyping LogicalRelation Properties Reduction LRInduction.
 Set Universe Polymorphism.
 
@@ -5,289 +6,186 @@ Definition escape0 {Γ A} :
     [Γ ||-< zero | A ] ->
     [Γ |- A].
 Proof.
-    intros.
-    destruct X.
-    eapply (LR_rec0 Γ A). exact valid.
-    + intros. destruct neA.
-      destruct D. assumption.
-    + intros. destruct H0. cbn in *.
-      destruct (D'_ emptyName).
-      assumption.
-Defined.
+  destruct 1.
+  eapply (LR_rect0 (fun Γ A _ _ _ _ => [Γ |- A])).
+  3: eassumption.
+  - intros ? ? neA.
+    now destruct neA as [? []].
+  - intuition.
+Qed.
 
 Definition escape1 {Γ A} :
     [Γ ||-< one | A ] ->
     [Γ |- A].
 Proof.
-    intros.
-    destruct X.
-    refine (LR_rec1 Γ A _ _ _ valid 
-      (fun Γ A T T0 T1 H => 
-        [Γ ||-< zero | A] ->
-        [Γ |- A]) 
-      (fun Γ A T T0 T1 H => 
-        [Γ ||-< one | A] ->
-        [Γ |- A]) _ _ _ _ _ _ _).
-    1, 4 : intros; destruct neA;
-      destruct D; exact wfA.
-    1, 3 : intros; destruct H0; 
-      destruct (D'_ emptyName);
-      assumption.
-    + intros.
-      constructor. assumption.
-    + intros.
-      eapply X.
-      exact H.
-    + econstructor; eassumption.
-Defined.
+  intros [? ? ? valid].
+  red in valid ; cbn in *.
+  eapply (LR_rect1' (fun Γ A _ _ _ _ => [Γ |- A]) (fun Γ A _ _ _ _ => [Γ |- A])).
+  6: eassumption.
+  - intros.
+    eapply escape0.
+    logrel.
+  - intros ? [].
+    mltt.
+  - intros ? ? [].
+    now destruct red.
+  - intros ? ? [].
+    now destruct red.
+  - easy.
+Qed.
 
 Definition escapeEqNe {Γ0 A0 B} : forall (neA : [Γ0 ||-ne A0]),
     [Γ0 ||-ne A0 ≅ B | neA] ->
     [Γ0 |- A0 ≅ B].
 Proof.
-    intros. destruct neA.
-    destruct X.
-    pose proof (TypeRedWFConv D).
-    pose proof (TypeSym (TypeRedWFConv D')).
-    eapply TypeTrans. eassumption.
-    eapply TypeTrans. eassumption.
-    eassumption.
+    intros [] [] ; cbn in *.
+    do 2 eapply TypeTrans.
+    all: mltt.
 Defined.
 
-Definition escapeEqPi {Γ0 A0} l : forall (H0 : [Γ0 ||-0Π A0]) 
-    (H1 : TyPiRel1 (LR (recl l)) H0),
-    (forall (Δ : PCUICAst.PCUICEnvironment.context) (h : [  |- Δ])
-       (B : PCUICAst.term), LogicalRelation.relEq (_F H0 h) B -> [Δ |- F H0 ≅ B]) ->
-    (forall (Δ : PCUICAst.PCUICEnvironment.context) (a : PCUICAst.term)
-       (h1 : [  |- Δ])
-       (h2 : [Δ ||-1 a ::: F H0 | {| valid := _F1 H1 h1 |}])
-       (B : PCUICAst.term),
-     LogicalRelation.relEq (_G H0 h1 h2) B ->
-     [Δ |- PCUICAst.subst1 a 0 (G H0) ≅ B]) ->
-    forall B, [Γ0 ||-1Π A0 ≅ B | H0] -> [Γ0 |- A0 ≅ B].
+Definition escapeEqPi {Γ A} : forall (ΠA : [Γ ||-Πr A]),
+    forall B, [Γ ||-Π A ≅ B | ΠA] -> [Γ |- A ≅ B].
 Proof.
-    intros. destruct H0.
-    pose proof (TypeRedWFConv (D'_ emptyName)).
-    eapply TypeTrans. eassumption.
-    destruct X1.
-    pose proof (TypeRedWFConv (D'' emptyName)).
-    eapply TypeTrans.
-    2 : exact (TypeSym X1).
-    exact (AeqB _ _).
+  intros [] ? [].
+  do 2 eapply TypeTrans.
+  all: mltt.
 Defined.
 
-Definition escapeEq0 {Γ A B H} :
+Definition escapeEq0 {Γ A B} (H : [Γ ||-< zero | A]) :
     [ Γ ||-< zero | A ≅ B | H ] ->
     [Γ |- A ≅ B].
 Proof.
-    intros.
-    destruct H.
-    revert B X.
-    eapply (LR_rec0 Γ A _ _ _ valid
-      (fun Γ A T T0 T1 H => forall B : PCUICAst.term,
-        [Γ ||-< zero | A ≅ B | LRValidMk _ _ _ H] -> 
-        [Γ |- A ≅ B])).
-    + intros; now eapply escapeEqNe. 
-    + intros; now eapply (escapeEqPi zero).
-    Unshelve.
-    all : assumption.
+  eapply (LR_rect0
+    (fun Γ A T T0 T1 H => forall B : term,
+      [Γ ||-< zero | A ≅ B | Build_LRValid H] -> 
+      [Γ |- A ≅ B])).
+  + intros; now eapply escapeEqNe. 
+  + intros; now eapply escapeEqPi.
 Defined.
 
-Definition escapeEq1 {Γ A B H} :
+Definition escapeEq1 {Γ A B} (H : [Γ ||-< one | A]) :
     [ Γ ||-< one | A ≅ B | H ] ->
     [Γ |- A ≅ B].
 Proof.
-    intros.
-    destruct H.
-    revert B X.
-    eapply (LR_rec1 Γ A _ _ _ valid
-      (fun Γ A T T0 T1 H => forall B : PCUICAst.term,
-        [Γ ||-< zero | A ≅ B | LRValidMk _ _ _ H] -> 
+    eapply (LR_rect1'
+      (fun Γ A T T0 T1 H => forall B : term,
+        [Γ ||-< zero | A ≅ B | Build_LRValid H] -> 
         [Γ |- A ≅ B])
-    (fun Γ A T T0 T1 H => forall B : PCUICAst.term,
-        [Γ ||-< one | A ≅ B | LRValidMk _ _ _  H] -> 
-        [Γ |- A ≅ B])).
-    all :cbn in *.
-    1, 4 : intros; now eapply escapeEqNe.
-    1 : intros; now eapply (escapeEqPi zero).
-    2 : intros; now eapply (escapeEqPi one).
-    + intros.
-      destruct H. rewrite Beq; constructor.
-      constructor. assumption.
-    + intros.
-      eapply X; eassumption.
-    Unshelve.
-    all : eassumption.
-Defined.
+    (fun Γ A T T0 T1 H => forall B : term,
+        [Γ ||-< one | A ≅ B | Build_LRValid H] -> 
+        [Γ |- A ≅ B])). 
+    all: cbn in *.
+    - intros.
+      now eapply (escapeEq0 (LRbuild lr)).
+    - intros ? [] _ [->].
+      mltt.
+    - intros ? ? [] ? [] ; cbn in *.
+      do 2 eapply TypeTrans.
+      all: mltt.
+    - intros.
+      now eapply escapeEqPi.
+    - eauto.
+Qed.
 
 Definition escapeTermNe {Γ0 A0 t}: forall
   (neA : [Γ0 ||-ne A0]),
   [Γ0 ||-ne t ::: A0 | neA] -> 
   [Γ0 |- t ::: A0].
 Proof.
-  intros. 
-  destruct neA.
-  destruct X.
-  gen_conv.
-  destruct X1.
-  exact (redFirstCTerm C).
+  intros [] [? []] ; cbn in *.
+  mltt.
 Defined.
 
-Definition escapeTermPi {Γ0 A0} l : forall   
-  (H0 : [Γ0 ||-0Π A0]) 
-  (H1 : TyPiRel1 (LR (recl l)) H0),
-  (forall (Δ : PCUICAst.PCUICEnvironment.context) 
-     (h : [  |- Δ]) (t : PCUICAst.term),
-   LogicalRelation.relTerm (_F H0 h) t -> [Δ |- t ::: F H0]) ->
-  (forall (Δ : PCUICAst.PCUICEnvironment.context) 
-     (a : PCUICAst.term) (h1 : [  |- Δ])
-     (h2 : [Δ ||-1 a ::: F H0 | {|  valid := _F1 H1 h1 |}])
-     (t : PCUICAst.term),
-   LogicalRelation.relTerm (_G H0 h1 h2) t ->
-   [Δ |- t ::: PCUICAst.subst1 a 0 (G H0)]) ->
-  forall t : PCUICAst.term, 
-  [Γ0 ||-1Π t ::: A0 | H0] -> 
-  [Γ0 |- t ::: A0].
+Definition escapeTermPi {Γ A} : forall (ΠA : [Γ ||-Πr A]) (t : term), 
+  [Γ ||-Π t ::: A | ΠA] -> 
+  [Γ |- t ::: A].
 Proof.
-  intros. destruct H0.      
-  destruct X1. cbn in *.
-  eapply wfTermConv.
-  destruct (redf emptyName).
-  exact wft.
-  exact (TypeSym (TypeRedWFConv (D'_ emptyName))).
+  intros [? ? ? ? []] ? [? []]; cbn in *.
+  mltt.
 Defined.
 
-Definition escapeTerm0 {Γ t A} : forall 
-    (H : [Γ ||-< zero | A ]),
-    [Γ ||-< zero | t ::: A | H ] ->
-    [Γ |- t ::: A].
+Definition escapeTerm0 {Γ t A} (H : [Γ ||-< zero | A ]) :
+  [Γ ||-< zero | t ::: A | H ] ->
+  [Γ |- t ::: A].
 Proof.
-    intros.
-    destruct H.
-    revert t X.
-    eapply (LR_rec0 Γ A _ _ _ valid
-      (fun Γ A T T0 T1 H => forall t : PCUICAst.term,
-        [Γ ||-< zero | t ::: A | LRValidMk _ _ _ H] -> 
-        [Γ |- t ::: A])).
-    + intros. now eapply escapeTermNe.
-    + intros. now eapply (escapeTermPi zero).
-    Unshelve.
-    all : assumption.
+  eapply (LR_rect0
+    (fun Γ A T T0 T1 H => forall t : term,
+      [Γ ||-< zero | t ::: A | Build_LRValid H] -> 
+      [Γ |- t ::: A])).
+  all: eauto using escapeTermNe, escapeTermPi.
 Defined.
 
-Definition escapeTerm1 {Γ t A} : forall 
-    (H : [Γ ||-< one | A ]),
-    [Γ ||-< one | t ::: A | H ] ->
-    [Γ |- t ::: A].
+Definition escapeTerm1 {Γ t A} (H : [Γ ||-< one | A ]) :
+  [Γ ||-< one | t ::: A | H ] ->
+  [Γ |- t ::: A].
 Proof.
-    intros.
-    destruct H.
-    revert t X.
-    eapply (LR_rec1 Γ A _ _ _ valid
-      (fun Γ A T T0 T1 H => forall t : PCUICAst.term,
-        [Γ ||-< zero | t ::: A | LRValidMk _ _ _  H] -> 
-        [Γ |- t ::: A])
-        (fun Γ A T T0 T1 H => forall t : PCUICAst.term,
-        [Γ ||-< one | t ::: A | LRValidMk _ _ _  H] -> 
-        [Γ |- t ::: A])).
-    1, 4 : intros; now eapply escapeTermNe.
-    1 : intros; now eapply (escapeTermPi zero).
-    2 : intros; now eapply (escapeTermPi one).
-    + intros. cbn in *.
-      destruct X.
-      exact (redFirstCWFTerm dd).
-    + intros. cbn in *.
-      apply X; eassumption.
-    Unshelve.
-    all : eassumption.
+  eapply (LR_rect1'
+    (fun Γ A T T0 T1 H => forall t : term,
+      [Γ ||-< zero | t ::: A | Build_LRValid H] -> 
+      [Γ |- t ::: A])
+      (fun Γ A T T0 T1 H => forall t : term,
+      [Γ ||-< one | t ::: A | Build_LRValid H] -> 
+      [Γ |- t ::: A])).
+  all: cbn.
+  - intros.
+    now eapply (escapeTerm0 (LRbuild lr)).
+  - intuition.
+  - eauto using escapeTermNe.
+  - eauto using escapeTermPi.
+  - auto.
 Defined.
 
-Definition escapeEqTermNe {Γ0 A0 t u}: forall  
+Definition escapeEqTermNe {Γ0 A0 t u}: forall
   (neA : [Γ0 ||-ne A0]),
   [Γ0 ||-ne t ≅ u ::: A0 | neA] -> 
   [Γ0 |- t ≅ u ::: A0].
 Proof.
-  intros.
-  destruct X.
-  destruct kNFEqm.
-  eapply TermTrans.
-  exact (RedConvTeWFC d').
-  eapply TermTrans. exact kEqm.
-  exact (TermSym (RedConvTeWFC d'')).
+  intros [] [? ? [] [] []].
+  do 2 eapply TermTrans.
+  all: mltt.
 Defined.
 
-Definition escapeEqTermPi {Γ0 A0} l : forall 
-  (H0 : [Γ0 ||-0Π A0]) (H1 : TyPiRel1 (LR (recl l)) H0),
-  (forall Δ (h : [  |- Δ]) t u,
-   LogicalRelation.relEqTerm (_F H0 h) t u -> [Δ |- t ≅ u ::: F H0]) ->
-  (forall Δ a
-     (h1 : [  |- Δ])
-     (h2 : [Δ ||-1 a ::: F H0 | {|valid := _F1 H1 h1 |}])
-     t u,
-   LogicalRelation.relEqTerm (_G H0 h1 h2) t u ->
-   [Δ |- t ≅ u ::: PCUICAst.subst1 a 0 (G H0)]) ->
-  forall t u,
-  [Γ0 ||-1Π t ≅ u ::: A0 | H0] -> 
-  [Γ0 |- t ≅ u ::: A0].
+Definition escapeEqTermPi {Γ A} : forall (ΠA: [Γ ||-Πr A]) t u,
+  [Γ ||-Π t ≅ u ::: A | ΠA] -> 
+  [Γ |- t ≅ u ::: A].
 Proof.
-  intros.
-  destruct X1.
-  destruct H0. cbn in *.
-  eapply TermConv.
-  2 : exact (TypeSym (TypeRedWFConv (D'_ emptyName))).
-  eapply TermTrans.
-  exact (RedConvTeWFC (redf' emptyName)).
-  eapply TermTrans.
-  exact (fEqg emptyName).
-  exact (TermSym (RedConvTeWFC (redg' emptyName))).
+  intros [? ? ? ? []] ? ? [? ? [] [] ? ? ?] ; cbn in *.
+  eapply (TermTrans (t' := nfL)).
+  1: mltt.
+  assert [Γ |- redPi ≅ A] by mltt.
+  eapply (TermTrans (t' := nfR)).
+  all: mltt.
 Defined.
 
-Definition escapeEqTerm0 {Γ t u A} : forall 
-    (H : [Γ ||-< zero | A ]),
-    [Γ ||-< zero | t ≅ u ::: A | H ] ->
-    [Γ |- t ≅ u::: A].
+Definition escapeEqTerm0 {Γ t u A} (H : [Γ ||-< zero | A ]) :
+  [Γ ||-< zero | t ≅ u ::: A | H ] ->
+  [Γ |- t ≅ u::: A].
 Proof.
-  intros.
-  destruct H.
-  revert t u X.
-  eapply (LR_rec0 Γ A _ _ _ valid
+  eapply (LR_rect0
   (fun Γ A T T0 T1 H => forall t u,
-    [Γ ||-< zero | t ≅ u ::: A | LRValidMk _ _ _ H] -> 
+    [Γ ||-< zero | t ≅ u ::: A | Build_LRValid H] -> 
     [Γ |- t ≅ u ::: A])).
-  cbn in *.
-  + intros; now eapply escapeEqTermNe.
-  + intros; eapply (escapeEqTermPi zero).
-  Unshelve.
-  all : eassumption.
+  all: eauto using escapeEqTermNe, escapeEqTermPi.
 Defined.
 
-Definition escapeEqTerm1 {Γ t u A} : forall 
-    (H : [Γ ||-< one | A ]),
-    [Γ ||-< one | t ≅ u ::: A | H ] ->
-    [Γ |- t ≅ u::: A].
+Definition escapeEqTerm1 {Γ t u A} (H : [Γ ||-< one | A ]) :
+  [Γ ||-< one | t ≅ u ::: A | H ] ->
+  [Γ |- t ≅ u::: A].
 Proof.
-  intros.
-  destruct H.
-  revert t u X.
-  eapply (LR_rec1 Γ A _ _ _ valid
+  eapply (LR_rect1'
   (fun Γ A T T0 T1 H => forall t u,
-    [Γ ||-< zero | t ≅ u ::: A | LRValidMk _ _ _ H] -> 
+    [Γ ||-< zero | t ≅ u ::: A | Build_LRValid H] -> 
     [Γ |- t ≅ u ::: A])
   (fun Γ A T T0 T1 H => forall t u,
-    [Γ ||-< one | t ≅ u ::: A | LRValidMk _ _ _ H] -> 
+    [Γ ||-< one | t ≅ u ::: A | Build_LRValid H] -> 
     [Γ |- t ≅ u ::: A])).
-  1, 4 : intros; now eapply escapeEqTermNe.
-  1 : intros; now eapply (escapeEqTermPi zero).
-  2 : intros; now eapply (escapeEqTermPi one).
-  + intros.
-    destruct X.
-    eapply TermTrans.
-    exact (RedConvTeWFC d_).
-    eapply TermTrans.
-    exact AeqBU.
-    exact (TermSym (RedConvTeWFC dd')).
-  + intros. cbn in *.
-    eapply X; try eassumption.
-  Unshelve.
-  all : eassumption.
+  all: cbn in *.
+  - intros.
+    now eapply (escapeEqTerm0 (LRbuild lr)).
+  - intros ? [] ? ? [] ; cbn in *.
+    do 2 eapply TermTrans.
+    all: mltt.
+  - eauto using escapeEqTermNe.
+  - eauto using escapeEqTermPi.
+  - eauto.
 Defined.
